src/ReactorModel/Determinism/Execution.lean
@@ -1,19 +1,18 @@
 import ReactorModel.Determinism.ExecutionStep
 
-theorem Execution.tag_le (e : s₁ ⇓* s₂) : s₁.ctx.tag ≤ s₂.ctx.tag := by
+theorem Execution.tag_le (e : s₁ ⇓* s₂) : s₁.tag ≤ s₂.tag := by
   induction e with
   | refl => simp
   | step h _ hi => exact le_trans h.tag_le hi
 
-theorem Execution.seq_currentProcessedRcns_ssubset_or_tag_lt : (s₁ ⇓ s₂) → (s₂ ⇓* s₃) → 
-    (s₁.ctx.currentProcessedRcns ⊂ s₃.ctx.currentProcessedRcns) ∨ (s₁.ctx.tag < s₃.ctx.tag)
+theorem Execution.seq_progress_ssubset_or_tag_lt : 
+    (s₁ ⇓ s₂) → (s₂ ⇓* s₃) → (s₁.progress ⊂ s₃.progress) ∨ (s₁.tag < s₃.tag)
   | e₁₂,        .step e e' => .inr $ lt_of_lt_of_le (e₁₂.seq_tag_lt e) e'.tag_le
-  | .close e,   .refl      => .inl $ e.currentProcessedRcns_ssubset
+  | .close e,   .refl      => .inl $ e.progress_ssubset
   | .advance a, .refl      => .inr $ a.tag_lt
 
-protected theorem Execution.deterministic : (s ⇓* s₁) → (s ⇓* s₂) → 
-    (s₁.ctx.tag = s₂.ctx.tag) → (s₁.ctx.currentProcessedRcns = s₂.ctx.currentProcessedRcns) → 
-    s₁ = s₂ := by
+protected theorem Execution.deterministic : 
+    (s ⇓* s₁) → (s ⇓* s₂) → (s₁.tag = s₂.tag) → (s₁.progress = s₂.progress) → s₁ = s₂ := by
   intro he₁ he₂ ht hc
   induction he₁ <;> cases he₂ 
   case refl.refl => rfl
@@ -21,10 +20,10 @@ protected theorem Execution.deterministic : (s ⇓* s₁) → (s ⇓* s₂) →
     rw [Execution.Step.deterministic h₁ₘ₁ h₁ₘ₂] at hi
     exact hi hₘ₂₂ ht hc
   case step.refl h₂₃ _ h₁₂ => 
-    match seq_currentProcessedRcns_ssubset_or_tag_lt h₁₂ h₂₃ with
+    match seq_progress_ssubset_or_tag_lt h₁₂ h₂₃ with
     | .inl h => exact absurd hc (Finset.ssubset_ne h).symm
     | .inr h => exact absurd ht (ne_of_lt h)
   case refl.step h₁₂ h₂₃ => 
-    match seq_currentProcessedRcns_ssubset_or_tag_lt h₁₂ h₂₃ with
+    match seq_progress_ssubset_or_tag_lt h₁₂ h₂₃ with
     | .inl h => exact absurd hc (Finset.ssubset_ne h)
     | .inr h => exact absurd ht (ne_of_lt h)
