src/ReactorModel/Determinism/ExecutionStep.lean
@@ -4,47 +4,43 @@ namespace Execution
 
 open State (Closed)
 
-theorem AdvanceTag.closed : (s₁ ⇓ₜ s₂) → Closed s₁
-  | mk _ h _ => h
-
-theorem AdvanceTag.not_Closed : (s₁ ⇓ₜ s₂) → ¬(Closed s₂)
-  | mk hg _ _, h => by
-    have h' := s₁.ctx.advanceTag_processedRcns_empty $ s₁.tag_lt_nextTag hg
-    exact absurd h' h.processedRcns_not_empty
-
-theorem AdvanceTag.nonrepeatable (a : s₁ ⇓ₜ s₂) : ¬(s₂ ⇓ₜ s₃) :=
-  (absurd ·.closed a.not_Closed)
-
-theorem AdvanceTag.tag_lt : (s₁ ⇓ₜ s₂) → s₁.ctx.tag < s₂.ctx.tag
-  | mk .. => by simp [Context.advanceTag_strictly_increasing]
-
-theorem AdvanceTag.determinisic : (s ⇓ₜ s₁) → (s ⇓ₜ s₂) → s₁ = s₂
-  | mk hg₁ _ hc₁, mk hg₂ _ hc₂ => by
-    simp only [hg₁, Option.some_inj] at hg₂
-    simp [clearingPorts_unique hc₁ hc₂, Context.advanceTag, hg₂]  
-
-theorem CompleteInstExecution.closed : (s₁ ⇓ᵢ| s₂) → Closed s₂
+theorem AdvanceTag.closed : (s₁ ⇓- s₂) → Closed s₁
   | mk _ h => h
 
-theorem CompleteInstExecution.not_Closed : (s₁ ⇓ᵢ| s₂) → ¬(Closed s₁)
+theorem AdvanceTag.not_Closed : (s₁ ⇓- s₂) → ¬(Closed s₂)
+  | mk hg _, h =>
+    absurd (s₁.ctx.advanceTag_progress_empty $ s₁.tag_lt_nextTag hg) h.progress_not_empty
+
+theorem AdvanceTag.nonrepeatable (a : s₁ ⇓- s₂) : ¬(s₂ ⇓- s₃) :=
+  (absurd ·.closed a.not_Closed)
+
+theorem AdvanceTag.tag_lt : (s₁ ⇓- s₂) → s₁.tag < s₂.tag
+  | mk .. => by simp [Context.advanceTag_strictly_increasing]
+
+theorem AdvanceTag.determinisic : (s ⇓- s₁) → (s ⇓- s₂) → s₁ = s₂
+  | mk hg₁ _, mk hg₂ _ => by simp [Option.some_inj.mp $ hg₂ ▸ hg₁]
+
+theorem ClosedExecution.closed : (s₁ ⇓| s₂) → Closed s₂
+  | mk _ h => h
+
+theorem ClosedExecution.not_Closed : (s₁ ⇓| s₂) → ¬(Closed s₁)
   | mk e _ => e.not_Closed
 
-theorem CompleteInstExecution.nonrepeatable (e : s₁ ⇓ᵢ| s₂) : ¬(s₂ ⇓ᵢ| s₃) :=
+theorem ClosedExecution.nonrepeatable (e : s₁ ⇓| s₂) : ¬(s₂ ⇓| s₃) :=
   (absurd e.closed ·.not_Closed)
 
-theorem CompleteInstExecution.currentProcessedRcns_ssubset :
-  (s₁ ⇓ᵢ| s₂) → s₁.ctx.currentProcessedRcns ⊂ s₂.ctx.currentProcessedRcns
-  | mk e _ => e.currentProcessedRcns_ssubset
+theorem ClosedExecution.progress_ssubset : (s₁ ⇓| s₂) → s₁.progress ⊂ s₂.progress
+  | mk e _ => e.progress_ssubset
 
-theorem CompleteInstExecution.rcns_eq : (s ⇓ᵢ| s₁) → (s ⇓ᵢ| s₂) → s₁.rtr.ids .rcn = s₂.rtr.ids .rcn
+theorem ClosedExecution.rcns_eq : (s ⇓| s₁) → (s ⇓| s₂) → s₁.rtr.ids .rcn = s₂.rtr.ids .rcn
   | mk e₁ _, mk e₂ _ => by 
     simp [Finset.ext_iff, Reactor.ids_mem_iff_obj?, ←e₁.preserves_rcns, e₂.preserves_rcns]
 
-theorem CompleteInstExecution.tag_eq : (s₁ ⇓ᵢ| s₂) → s₁.ctx.tag = s₂.ctx.tag
+theorem ClosedExecution.tag_eq : (s₁ ⇓| s₂) → s₁.tag = s₂.tag
   | mk e _ => e.tag_eq
 
-theorem CompleteInstExecution.convergent_ctx : 
-  (s ⇓ᵢ| s₁) → (s ⇓ᵢ| s₂) → s₁.ctx = s₂.ctx := by
+theorem ClosedExecution.convergent_ctx : 
+  (s ⇓| s₁) → (s ⇓| s₂) → s₁.ctx = s₂.ctx := by
   intro hc₁ hc₂
   ext1
   apply Finmap.ext
@@ -52,22 +48,22 @@ theorem CompleteInstExecution.convergent_ctx :
   have hc₁₂ := hc₁.rcns_eq hc₂
   cases hc₁ with | mk e₁ hc₁ => 
   cases hc₂ with | mk e₂ hc₂ => 
-  by_cases hg : g = s.ctx.tag
+  by_cases hg : g = s.tag
   case pos => 
     have h₁ := hc₁ |> Option.some_inj.mpr
     have h₂ := hc₂ |> Option.some_inj.mpr
-    rw [Context.currentProcessedRcns_def] at h₁ h₂
+    rw [Context.progress_def] at h₁ h₂
     simp only [←e₁.tag_eq, ←e₂.tag_eq, ←hg] at h₁ h₂
     simp only [h₁, h₂, hc₁₂]
   case neg => simp only [←e₁.preserves_ctx_past_future g hg, e₂.preserves_ctx_past_future g hg]
 
-theorem CompleteInstExecution.deterministic : (s ⇓ᵢ| s₁) → (s ⇓ᵢ| s₂) → s₁ = s₂
+theorem ClosedExecution.deterministic : (s ⇓| s₁) → (s ⇓| s₂) → s₁ = s₂
   | i₁@(mk e₁ _), i₂@(mk e₂ _) => e₁.deterministic e₂ $ i₁.convergent_ctx i₂
 
-theorem CompleteInstExecution.not_AdvanceTag : (s ⇓ᵢ| s₁) → ¬(s ⇓ₜ s₂) := 
-  fun ⟨e, _⟩ ⟨_, h, _⟩ => absurd h e.not_Closed
+theorem ClosedExecution.not_AdvanceTag : (s ⇓| s₁) → ¬(s ⇓- s₂) := 
+  fun ⟨e, _⟩ ⟨_, h⟩ => absurd h e.not_Closed
 
-theorem Step.tag_le : (s₁ ⇓ s₂) → s₁.ctx.tag ≤ s₂.ctx.tag
+theorem Step.tag_le : (s₁ ⇓ s₂) → s₁.tag ≤ s₂.tag
   | close e   => le_of_eq e.tag_eq
   | advance a => le_of_lt a.tag_lt
 
@@ -76,7 +72,7 @@ protected theorem Step.deterministic : (s ⇓ s₁) → (s ⇓ s₂) → s₁ = 
   | advance a₁, advance a₂                  => a₁.determinisic a₂
   | close e, advance a | advance a, close e => absurd a e.not_AdvanceTag
 
-theorem Step.seq_tag_lt : (s₁ ⇓ s₂) → (s₂ ⇓ s₃) → s₁.ctx.tag < s₃.ctx.tag
+theorem Step.seq_tag_lt : (s₁ ⇓ s₂) → (s₂ ⇓ s₃) → s₁.tag < s₃.tag
   | advance a₁, advance a₂ => absurd a₂ a₁.nonrepeatable 
   | close e₁,   close e₂   => absurd e₂ e₁.nonrepeatable
   | advance a,  close e    => e.tag_eq ▸ a.tag_lt
